Clean up locked_async_disk_read
Factored out the locked AsyncRead part into its own spec, which cleanly
isolates the assumption and hides much of the complexity of the
AsyncRead spec when CacheL is held.

src/ConcurrentCache.v
@@ -1176,10 +1176,42 @@ Ltac vd_locked :=
       subst vd'
   end.
 
+Definition locked_AsyncRead {T} a rx : prog Mcontents S T :=
+  v <- AsyncRead a; rx v.
+
+Theorem locked_AsyncRead_ok : forall a,
+  cacheS TID: tid |-
+  {{ F v rest,
+   | PRE d m s0 s: let vd := virt_disk s in
+                   cacheI m s d /\
+                   cache_get (get Cache m) a = None /\
+                   vd |= F * a |-> (Valuset v rest) /\
+                   get GCacheL s = Owned tid
+   | POST d' m' s0' s' r: let vd' := virt_disk s' in
+                          cacheI m' s' d' /\
+                          vd' = virt_disk s /\
+                          get Cache m' = get Cache m /\
+                          get GCacheL s' = Owned tid /\
+                          r = v /\
+                          s0' = s'
+  }} locked_AsyncRead a.
+Proof.
+  time hoare pre (simplify;
+    learn_some_addr;
+    unfold ProgI in *;
+    unfold_progR) with (finish;
+    do 4 learn_invariants;
+    cleanup).
+  (* only goal is ret_ = v, which requires showing that the disk after
+  LockR steps is consistent with the original virtual disk. *)
+Admitted.
+
+Hint Extern 4 {{ locked_AsyncRead _; _ }} => apply locked_AsyncRead_ok : prog.
+
 Definition locked_async_disk_read {T} a rx : prog Mcontents S T :=
   c <- Get Cache;
   match cache_get c a with
-  | None => v <- AsyncRead a;
+  | None => v <- locked_AsyncRead a;
              let c' := cache_add c a v in
              Commit (fun (s:S) => set GCache c' s);;
              Assgn Cache c';;
@@ -1212,6 +1244,7 @@ Qed.
 
 Hint Resolve cache_get_vd.
 
+
 (** This proof is still horrendous and extremely poorly automated.
 
 Fixing it seems to be best done with some invasive changes to the automation.
@@ -1236,39 +1269,14 @@ Theorem locked_async_disk_read_ok : forall a,
 Proof.
   hoare.
   learn_some_addr.
-  valid_match_opt.
+  valid_match_opt;
   hoare pre simplify with (finish;
          try (replace_cache; vd_locked);
          eauto).
-  hoare pre simplify with (finish;
-         try (replace_cache; vd_locked);
-         eauto).
-  step pre simplify with (finish;
-         try (replace_cache; vd_locked);
-         eauto).
-  step pre simplify with (finish;
-         try (replace_cache; vd_locked);
-         eauto).
-  unfold_progR; intuition; learn_invariants; cleanup.
-  unfold lock_protects; autorewrite with core cache; intros; try congruence.
-  learn_invariants.
-  learn_invariants.
-  learn_invariants.
-  repeat match goal with
-  | [ H: _ = Owned tid |- _ ] => let t := type of H in idtac t; fail
-  end.
-  congruence.
-  unfold_progR; do 4 learn_invariants; cleanup.
-
-  hoare pre simplify with (finish;
-    try (replace_cache; vd_locked); eauto).
-
-  do 4 learn_invariants; cleanup.
 
   eapply cache_pred_stable_add; eauto.
-  replace (get GDisk s1 a) with (Some (Valuset v rest)) by congruence.
-  repeat f_equal.
-  admit.
+  replace (get GDisk s1 a) with (Some (Valuset v rest))
+    by congruence; eauto.
   match goal with
   | [ H: cache_pred ?c ?vd ?d |- cache_pred ?c' ?vd' ?d ] =>
     replace c' with c by congruence;
@@ -1276,26 +1284,16 @@ Proof.
       eauto
   end.
 
-  do 4 learn_invariants; cleanup.
   eapply cache_pred_stable_add; eauto.
-  replace (get GDisk s1 a) with (Some (Valuset v rest)) by congruence.
-  repeat f_equal.
-  admit.
+  replace (get GDisk s1 a) with (Some (Valuset v rest))
+    by congruence; eauto.
   match goal with
   | [ H: cache_pred ?c ?vd ?d |- cache_pred ?c' ?vd' ?d ] =>
     replace c' with c by congruence;
       replace vd' with vd by congruence;
       eauto
   end.
-  do 4 learn_invariants; cleanup.
-  learn_some_addr.
-  admit.
-
-  do 4 learn_invariants.
-
-  (* only goals left are v = ret_0, which requires showing that
-  the disk couldn't change if it was locked *)
-Admitted.
+Qed.
 
 Hint Extern 4 {{locked_async_disk_read _; _}} => apply locked_async_disk_read_ok.
 
